Lech/SetP/BasisEmptyP.lean
@@ -185,10 +185,10 @@ theorem denoteP_emptyRecA_type {m : EnvS2Core V env}
       rw [Lech.Env.find?_cons, if_neg (by decide)]; exact hE
     rw [denoteP_levelless_const hf (by rfl), hleaf]
   rw [show emptyRecA.toConstantVal.type
-      = Expr.forallE (Name.anonymous.str "motive")
-          (Expr.forallE (Name.anonymous.str "t") (.const emptyName [])
+      = Expr.forallE .anonymous
+          (Expr.forallE .anonymous (.const emptyName [])
             (.sort (.param uN)) { bi := .default, pw := .never })
-          (Expr.forallE (Name.anonymous.str "t") (.const emptyName [])
+          (Expr.forallE .anonymous (.const emptyName [])
             (.app (.bvar 1) (.bvar 0))
             { bi := .default, pw := .ifAllZero [uN] })
           { bi := .default, pw := .ifAllZero [uN] } from rfl]
@@ -292,10 +292,10 @@ theorem declBasisPB_emptyK {env₂ : Env} (mp : EnvS2PM V μ env)
       (fun _ _ heq => nomatch heq), (fun _ heq => nomatch heq)⟩
     show Expr.constsResolve _ emptyRecA.toConstantVal.type = true
     simp only [show emptyRecA.toConstantVal.type
-        = Expr.forallE (Name.anonymous.str "motive")
-            (Expr.forallE (Name.anonymous.str "t") (.const emptyName [])
+        = Expr.forallE .anonymous
+            (Expr.forallE .anonymous (.const emptyName [])
               (.sort (.param uN)) { bi := .default, pw := .never })
-            (Expr.forallE (Name.anonymous.str "t") (.const emptyName [])
+            (Expr.forallE .anonymous (.const emptyName [])
               (.app (.bvar 1) (.bvar 0))
               { bi := .default, pw := .ifAllZero [uN] })
             { bi := .default, pw := .ifAllZero [uN] } from rfl,
